
#+options: ':nil *:t -:t ::t <:t H:3 \n:nil ^:t arch:headline
#+options: author:t broken-links:nil c:nil creator:nil
#+options: d:(not "LOGBOOK") date:t e:t email:nil f:t inline:t num:t
#+options: p:nil pri:nil prop:nil stat:t tags:t tasks:t tex:t
#+options: timestamp:t title:t toc:nil todo:t |:t
#+title: sml-hw08-p01_a
#+date: \today
#+author: Ayam Banjade
#+language: en



\begin{align*}
  dX &= f(X,t)dt + g(X,t)dW \\
  F(X,t) &= (1+t)^2 \cos(X) 
\end{align*}

In the slides, we are given:

\begin{align*}
dF = \left[ \frac{\partial F}{\partial t} + \frac{\partial F}{\partial X} f + \frac{1}{2} \frac{\partial ^2 F}{\partial X^2} g^2 \right]dt + g \frac{\partial F}{\partial X} dW \\
\end{align*}

For geometric brownian motion: $f = \mu X(t)$ and $g = \sigma X(t)$ - where $X(t)$ is geometric Brownian motion (from Homework 7).

To make things easier:

\begin{align*}
\frac{\partial F}{\partial t} &= 2(1+t) \cos(X) \\
\frac{\partial F}{\partial X} &= -(1+t)^2 \sin(X) \\
\frac{\partial^2 F}{\partial X^2} &= -(1+t)^2 \cos(X) 
\end{align*}

Also:
\begin{align*}
\cos(X) &= \frac{F(X,t)}{(1+t)^2} \\
\sin^2(X) &= 1 - \frac{F(X,t)^2}{(1+t)^4} \\
\sin(X) &= \frac{\sqrt{(1+t)^4 - F(X,t)^2} }{(1+t)^2} \\
\end{align*}

Substituting values:
\begin{align*}
dF &= \left[ 2(1+t) \cos(X) -(1+t)^2 \sin(X) f - \frac{(1+t)^2}{2} \cos(X) g^2 \right]dt - g(1+t)^2 \sin(X) dW \\
&= \left[ 2 \frac{(1+t)^2}{(1+t)} \cos(X) - (1+t)^2 \sin(X) f - \frac{F}{2} g^2 \right]dt - g(1+t)^2 \sin(X) dW \\
&= \left[ \frac{2F}{1+t} - (1+t)^2 \sin(X) \mu X - \frac{F}{2} (\sigma X)^2 \right]dt - \sigma X (1+t)^2 \sin(X) dW \\
&= \left[ \frac{2F}{1+t} - (1+t)^2 \frac{\sqrt{(1+t)^4 - F(X,t)^2} }{(1+t)^2} \mu \cos^{-1} \left(\frac{F(X,t)}{(1+t)^2}\right) - \frac{F}{2} (\sigma \cos^{-1}\left( \frac{F(X,t)}{(1+t)^2} \right))^2 \right]dt \\
&- \sigma \cos^{-1}\left(\frac{F(X,t)}{(1+t)^2}\right) (1+t)^2 \frac{\sqrt{(1+t)^2 - F(X,t)}}{1+t} dW \\
&= \left[ \frac{2F}{1+t} - (1+t) \sqrt{(1+t)^2 - F(X,t)} \mu \cos^{-1} \left(\frac{F(X,t)}{(1+t)^2}\right) - \frac{F}{2} (\sigma \cos^{-1}\left( \frac{F(X,t)}{(1+t)^2} \right))^2 \right]dt \\
&- \sigma \cos^{-1}\left(\frac{F(X,t)}{(1+t)^2}\right) (1+t) \\sqrt{(1+t)^2 - F(X,t)} dW \\
\end{align*}
